if... almost there....

hoare_wp.fst
@@ -303,16 +303,16 @@ let proof_if_true c p1 p2 h =
   DImplIntro (FAnd (pif c p1 p2 h) (c h)) (p1 h) (proof_if_true_temp c p1 p2 h)
 
 val proof_if_false_temp : c : pred -> p1 : pred -> p2 : pred -> h : heap -> 
-                        lhs:deduce(FAnd (pif c p1 p2 h) (c h)) -> 
-                        Tot (deduce (p1 h))
+                        lhs:deduce(FAnd (pif c p1 p2 h) (fnot (c h))) -> 
+                        Tot (deduce (p2 h))
 let proof_if_false_temp c p1 p2 h lhs = 
-    let pc = DAndElim2 (pif c p1 p2 h) (c h) lhs in
-    let pcp1 = DAndElim1 ((pimpl c p1) h) ((pimpl (pnot c) p2) h) (DAndElim1 (pif c p1 p2 h) (c h) lhs) in
-    DImplElim (c h) (p1 h) pcp1 pc 
+    let pcf = DAndElim2 (pif c p1 p2 h) (fnot (c h)) lhs in
+    let pcp2 = DAndElim2 ((pimpl c p1) h) ((pimpl (pnot c) p2) h) (DAndElim1 (pif c p1 p2 h) (fnot (c h)) lhs) in
+    DImplElim (fnot (c h)) (p2 h) pcp2 pcf
 
-val proof_if_true : c : pred -> p1 : pred -> p2 : pred -> h : heap -> Tot (deduce( FImpl (pand (pif c p1 p2) c h ) (p1 h) ))
-let proof_if_true c p1 p2 h = 
-  DImplIntro (FAnd (pif c p1 p2 h) (c h)) (p1 h) (proof_if_false_temp c p1 p2 h)
+val proof_if_false : c : pred -> p1 : pred -> p2 : pred -> h : heap -> Tot (deduce( FImpl (pand (pif c p1 p2) (pnot c) h ) (p2 h) ))
+let proof_if_false c p1 p2 h = 
+  DImplIntro (FAnd (pif c p1 p2 h) (pnot c h)) (p2 h) (proof_if_false_temp c p1 p2 h)
 
 val plouf : q : pred -> h : heap -> deduce (q h) -> Tot (deduce (q h))
 let plouf q h p = p
@@ -333,33 +333,15 @@ let rec wlp_sound c q =
       let p = (pimpl (pand (pif (bpred be) (wlp ct q) (wlp ce q)) (bpred be)) (wlp ct q)) in
       let p' = wlp ct q in
       let hthen = hoare_consequence (pand (pif (bpred be) (wlp ct q) (wlp ce q)) (bpred be)) (wlp ct q) q q ct wlp_t vpp' (DForallIntro (pimpl q q) (fun (h:heap) -> (DImplIntro (q h) (q h) (plouf q h)))) in
-      //let helse = hoare_consequence (pand (pif (bpred be) (wlp ct q) (wlp ce q)) (bpred be)) (wlp ct q) q q ct wlp_t vpp' (DForallIntro (pimpl q q) (fun (h:heap) -> (DImplIntro (q h) (q h) (plouf q h)))) in
-      admit()
+      let vpp'' = DForallIntro (pimpl (pand (pif (bpred be) (wlp ct q) (wlp ce q)) (pnot (bpred be))) (wlp ce q)) (proof_if_false (bpred be) (wlp ct q) (wlp ce q)) in 
+      let helse = hoare_consequence (pand (pif (bpred be) (wlp ct q) (wlp ce q)) (pnot (bpred be))) (wlp ce q) q q ce wlp_e vpp'' (DForallIntro (pimpl q q) (fun (h:heap) -> (DImplIntro (q h) (q h) (plouf q h)))) in
+      hoare_if (pif (bpred be) (wlp ct q) (wlp ce q)) q be ct ce hthen helse
   | _ -> admit() (* need more definitions to prove the rest formally *)
 
 
 
+
 (*
-
-hoare_c (fun h -> FAnd (p h) (fnot (bpred be h))) e q
-
-val pimpl : pred -> pred -> Tot pred
-let pimpl p1 p2 h = FImpl (p1 h) (p2 h)
-
-val pred_impl : pred -> pred -> Tot form
-let pred_impl p q = FForall (pimpl p q)
-
-
-val hoare_consequence : p:pred -> p':pred -> q:pred -> q':pred -> c:com ->
-                        hoare_c p' c q'        -> 
-                        deduce (pred_impl p p') -> 
-                        deduce (pred_impl q' q) -> 
-                        Tot (hoare_c p c q)
-
-pand (pimpl pg pt) (pimpl (pnot pg) pe)
-
-((pg ==> pt) && (not pg ==> pe))
-
 val hoare_if : p:pred -> q:pred -> be:bexp -> t:com -> e:com ->
                 hoare_c (fun h -> FAnd (p h) (bpred be h))  t q ->
                 hoare_c (fun h -> FAnd (p h) (fnot (bpred be h))) e q ->
